code/Cse230wi25/full/L10Types.lean
@@ -1,0 +1,759 @@
+
+import Cse230wi25.L05Evidence
+
+set_option pp.fieldNotation false
+set_option pp.proofs true
+
+
+/- @@@
+
+# Type Soundness via Small-Step Semantics
+
+Next, lets look at a concrete application of *small-step* semantics: to prove the correctness of a type checker.
+
+## Floating IMP
+
+Our old `IMP` language has no type-safety issues because, well, every variable is simply a `Nat`.
+
+Let us extend the set of possible `Val` to include *floating* point values as well.
+
+@@@ -/
+
+
+inductive Val where
+  | Iv : Int -> Val
+  | Fv : Float -> Val
+  deriving Repr
+
+open Val
+
+/- @@@
+We can have *integer* values like
+@@@ -/
+
+#eval (Iv 12)
+
+/- @@@
+Or *floating point* values like
+@@@ -/
+
+#eval (Fv 3.14)
+
+
+/- @@@
+
+As before,
+
+- an *identifier* or *variable* `Vname` is just a `String` and
+- a `State` maps `Vname` to `Val` (which is either an `Int` or a `Float`).
+
+@@@ -/
+
+abbrev Vname := String
+
+abbrev State := Vname -> Val
+
+@[simp] def upd (s: State) (x: Vname) (v: Val) : State :=
+  λ y => if y = x then v else s y
+
+notation:10 s " [ " x " := " v " ] " => upd s x v
+
+/- @@@
+
+### Arithmetic and Boolean Expressions
+
+Finally, we can extend `Aexp` to include `Int` and `Float` constants, together with
+the usual binary operations as:
+
+@@@ -/
+
+
+
+inductive Aexp where
+  | Ic  : Int -> Aexp            -- integer constant
+  | Fc  : Float -> Aexp          -- floating point constant
+  | V   : Vname -> Aexp          -- variable
+  | Add : Aexp -> Aexp -> Aexp   -- addition
+  deriving Repr
+
+open Aexp
+
+inductive Bexp where
+  | Bc   : Bool -> Bexp
+  | Not  : Bexp -> Bexp
+  | And  : Bexp -> Bexp -> Bexp
+  | Less : Aexp -> Aexp -> Bexp
+  deriving Repr
+
+open Bexp
+
+
+
+class ToAexp (a : Type) where
+  toAexp : a -> Aexp
+
+
+instance : OfNat Aexp (n: Nat) where
+  ofNat := Ic n
+
+instance : ToAexp Int where
+  toAexp := Ic
+
+instance : ToAexp String where
+  toAexp := V
+
+instance : Add Aexp where
+  add := fun a1 a2 => Add a1 a2
+
+instance : HAdd String Aexp Aexp where
+  hAdd := fun s a => Add (V s) a
+
+instance : HAdd String Int Aexp where
+  hAdd := fun s a => Add (V s) (Ic a)
+
+def mkVar (s: String) (i : Nat) : Aexp := V (s!"{s}_{i}")
+
+notation:80 lhs:91 "#" rhs:90 => mkVar lhs rhs
+
+def x := "x"
+def y := "y"
+def z := "z"
+
+def aexp0 : Aexp := x#1 + y#1 + z#1 + 5
+
+#eval aexp0
+
+/- @@@
+
+### Evaluating Expressions
+
+Can you think about why it is a bit tedious (but not impossible!)
+to define `aval` for this new `Aexp`?
+
+So, instead lets define the evaluation of `Aexp` using
+an `inductive` predicate, where we need only define the
+cases where a value is produced and we can *omit* the
+cases where an `Int` is added to / compared against a `Float`.
+
+@@@ -/
+
+
+inductive Taval : Aexp -> State -> Val -> Prop where
+
+  | T_Ic  : ∀ {i s},
+            Taval (Ic i) s (Iv i)
+
+  | T_Rc  : ∀ {f s},
+            Taval (Fc f) s (Fv f)
+
+  | T_V   : ∀ {x s},
+            Taval (V x) s (s x)
+
+  | T_AddI : ∀ {a1 a2 s i1 i2},
+             Taval a1 s (Iv i1) -> Taval a2 s (Iv i2) ->
+             Taval (Add a1 a2) s (Iv (i1 + i2))
+
+  | T_AddF : ∀ {a1 a2 s r1 r2},
+             Taval a1 s (Fv r1) -> Taval a2 s (Fv r2) ->
+             Taval (Add a1 a2) s (Fv (r1 + r2))
+
+open Taval
+
+inductive Tbval : Bexp -> State -> Bool -> Prop where
+
+  | T_Bc  : ∀ {v s},
+            Tbval (Bc v) s v
+
+  | T_Not : ∀ {b v s},
+            Tbval b s v ->
+            Tbval (Not b) s (!v)
+
+  | T_And : ∀ {b1 b2 v1 v2 s},
+            Tbval b1 s v1 -> Tbval b2 s v2 ->
+            Tbval (And b1 b2) s (v1 && v2)
+
+  | T_LessI : ∀ {a1 a2 i1 i2 s},
+              Taval a1 s (Iv i1) -> Taval a2 s (Iv i2) ->
+              Tbval (Less a1 a2) s (i1 < i2)
+
+  | T_LessF : ∀ {a1 a2 r1 r2 s},
+              Taval a1 s (Fv r1) -> Taval a2 s (Fv r2) ->
+              Tbval (Less a1 a2) s (r1 < r2)
+
+open Tbval
+
+
+def st0 : State := fun x => match x with
+  | "x" => Iv 3
+  | "y" => Iv 4
+  | _   => Iv 0
+
+/- @@@
+
+### Floating Commands
+
+Next, as with plain IMP, we define the type `Com`
+of commands, now using the new `Aexp` and `Bexp`.
+
+@@@ -/
+
+inductive Com where
+  | Skip   : Com
+  | Assign : Vname -> Aexp -> Com
+  | Seq    : Com   -> Com  -> Com
+  | If     : Bexp  -> Com  -> Com -> Com
+  | While  : Bexp  -> Com  -> Com
+  deriving Repr
+
+open Com
+
+infix:10 "<<"  => fun x y => Less x y
+infix:10 "<~"  => Com.Assign
+infixr:8 ";;" => Com.Seq
+notation:10 "IF" b "THEN" c1 "ELSE" c2 => Com.If b c1 c2
+notation:12 "WHILE" b "DO" c "END" => Com.While b c
+
+/- @@@
+
+And we can define a `SmallStep` operational semantics
+for `Com` similar to that from the previous lecture.
+
+**NOTE** Instead of using the *functions* `aval` and `bval`
+we simply use the *relations* `Taval` and `Tbval`.
+
+@@@ -/
+
+abbrev Configuration := (Com × State)
+
+
+inductive Step : Configuration -> Configuration -> Prop where
+
+   | Assign : ∀ {x a s v},
+                Taval a s v ->
+                Step (x <~ a, s) (Skip, s [x := v])
+
+   | Seq1   : ∀ {c s},
+                Step ((Skip ;; c), s) (c, s)
+
+   | Seq2   : ∀ {c1 c1' c2 s s'},
+                Step (c1, s) (c1', s') ->
+                Step ((c1 ;; c2) , s) ((c1' ;; c2), s')
+
+   | IfTrue : ∀ {b c1 c2 s},
+                Tbval b s true ->
+                Step (IF b THEN c1 ELSE c2, s) (c1, s)
+
+   | IfFalse : ∀ {b c1 c2 s},
+                Tbval b s false ->
+                Step (IF b THEN c1 ELSE c2, s) (c2, s)
+
+   | While   : ∀ { b c s },
+                Step (Com.While b c, s) (Com.If b (c ;; (Com.While b c)) Skip, s)
+
+
+/- @@@
+
+### Getting Stuck / Going Wrong
+
+Now that we have `Int` and `Float` values, we have introduced the possibility
+of programs **going wrong**. For example, we have not defined the meaning of
+`Add (Ic 2) (Fc 3.1)` because doing so would require adding an `Int` and a
+`Float` which (suppose we don't have any "casting") is meaningless.
+
+In that case, a program like
+
+```
+x <~ Ic 2 ;;
+y <~ Fc 3.1 ;;
+z <~ x + y ;;
+...
+```
+
+is *also* meaningless because the addition would **get stuck**.
+
+How can we make sure that programs are "ok", that is, they **do not get stuck**?
+
+## Type Checking
+
+Well, this is precisely what **type checking** was invented to solve: to **predict** --
+right when you *write* your code, that under no circumstances would execution get stuck
+or go wrong because you mixed up the wrong values for some operation.
+
+### Types
+
+For our simple `FIMP` we require just two types "int" and "float" and so we can model
+these as a new (lean) type `Ty` with the constructors (values) `TInt` and `TFloat`
+
+@@@ -/
+
+inductive Ty where
+  | TInt : Ty
+  | TFloat : Ty
+  deriving Repr
+
+/- @@@
+
+### Environments
+
+Next, we need a *table* or a *map* that records the `Ty` for each program variable.
+Often this structure is called a **Type `Environment`** and in PL papers, written
+using the letter `Γ`
+
+@@@ -/
+
+
+open Ty
+
+abbrev Env := Vname -> Ty
+
+/- @@@
+For example, here is an `Env`ironment where *every* variable is presumed to be an integer.
+@@@ -/
+
+@[simp] def Γᵢ : Env := fun _ => TInt
+
+
+/- @@@
+
+### Typing Judgments
+
+In Floyd-Hoare logic we proved propositions of the form `{p} c {q}`
+that said, roughly, that
+
+**IF**
+
+- we start execution in a *pre-state* where `p` was true and
+- execution of `c` terminates in some *post-state*
+
+**THEN**
+
+- the *post-state* will satisfy the assertion `q`
+
+
+Similarly, with type systems we will prove propositions
+of the form `Γ ⊢ e : τ` which say that
+
+**IF**
+
+- the variables in `e` are assumed to have the types given in `Γ`
+
+**THEN**
+
+- the expression `e` can be determined to have the type `τ`
+
+We say that `e` **has-type** `τ` in environment `Γ`.
+
+### Typing Rules for Arithmetic Expressions
+
+Next, lets write down some **rules** that establish this `HasType` relation,
+for each of the different kinds of `Aexp` and `Bexp`. The rules should let
+us establish the proposition that `Γᵢ ⊢ x + (10 + y) : int` i.e. `x + (10 + y)` has
+the type `int` in an environment where all the variables are of type `int`.
+
+We want the rules to be **syntax-directed** meaning a **single rule** should
+apply for each kind of expression. (Why?)
+
+
+```
+
+----------------[int]
+Γ ⊢ 3 : ???
+
+
+----------------[float]
+Γ ⊢ 3.14 : ???
+
+
+----------------[var]
+Γ ⊢ x : ???
+
+
+--------------------[add]
+Γ ⊢ a1 + a2 : ???
+```
+
+@@@ -/
+
+
+inductive HasTyA : Env -> Aexp -> Ty -> Prop where
+
+  | Ty_Ic : ∀ {Γ i},
+            HasTyA Γ (Ic i) TInt
+
+  | Ty_Fc : ∀ {Γ r},
+            HasTyA Γ (Fc r) TFloat
+
+  | Ty_V  : ∀ {Γ x},
+            HasTyA Γ (V x) (Γ x)
+
+  | Ty_AddI : ∀ {Γ a1 a2},
+              HasTyA Γ a1 TInt -> HasTyA Γ a2 TInt ->
+              HasTyA Γ (Add a1 a2) TInt
+
+  | Ty_AddF : ∀ {Γ a1 a2},
+              HasTyA Γ a1 TFloat -> HasTyA Γ a2 TFloat ->
+              HasTyA Γ (Add a1 a2) TFloat
+
+
+notation:10 Γ " ⊢ " a " : " τ => HasTyA Γ a τ
+
+/- @@@
+
+Let us check our example
+
+                      -------------[int]    -------------[var]
+                      Γᵢ ⊢ 10 : int         Γᵢ ⊢ y : int
+------------[var]     -----------------------------------[addI]
+Γᵢ ⊢ x : int          Γᵢ ⊢ (10 + y) : int
+-----------------------------------------[addI]
+Γᵢ ⊢ x + (10 + y) : int
+
+Lets see why having **syntax directed** rules is useful!
+
+@@@ -/
+
+example : Γᵢ ⊢ (V x + (Ic 10 + V y)) : TInt := by
+  sorry
+
+
+
+/- @@@
+### Typing Rules for Boolean Expressions
+
+Next, lets work out the rules for `Bexp` -- here we can just write
+`Γ ⊢ b` (and leave out `: bool` because?)
+
+
+```
+???
+---------------
+Γ ⊢ true : ???
+
+
+???
+---------------[not]
+Γ ⊢ ¬ b : ???
+
+
+???
+-------------------[and]
+Γ ⊢ b1 /\ b2 : ???
+
+???
+--------------------[less]
+Γ ⊢ a1 < a2 : ???
+```
+@@@ -/
+
+
+inductive HasTyB : Env -> Bexp -> Prop where
+  | Ty_Bc   : ∀ {Γ v},
+              HasTyB Γ (Bc v)
+
+  | Ty_Not  : ∀ {Γ b},
+              HasTyB Γ b ->
+              HasTyB Γ (Not b)
+
+  | Ty_And  : ∀ {Γ b1 b2},
+              HasTyB Γ b1 -> HasTyB Γ b2 ->
+              HasTyB Γ (And b1 b2)
+
+  | Ty_Less : ∀ {Γ a1 a2 t} ,
+              HasTyA  Γ a1 t -> HasTyA Γ a2 t ->
+              HasTyB Γ (Less a1 a2)
+
+notation:10 Γ " ⊢ " a  => HasTyB Γ a
+
+/- @@@
+
+Again, the **syntax-directed** nature of the rules
+makes establishing the "has-type" facts super easy!
+
+@@@ -/
+
+example : Γᵢ ⊢ (V x + (Ic 10 + V y)) << Ic 29 := by
+  sorry
+
+/- @@@
+
+### Typing Rules for Commands
+
+Finally, lets work out the rules for typing commands.
+
+What does the **typing judgment** for a command look like?
+
+#### QUIZ
+
+Should we the following hold?
+
+```
+Γᵢ ⊢ x <~ 10 ;; Skip ;; y <~ 10 ;; z <~ x + y
+```
+
+#### QUIZ
+
+```
+Γᵢ ⊢ x <~ 10 ;; Skip ;; y <~ 1.0 ;; z <~ x + y
+```
+
+What should the rules look like so that we can establish / reject appropriately?
+
+
+@@@ -/
+
+inductive HasTyC : Env -> Com -> Prop where
+  | Ty_Skip   : ∀ {Γ},
+                HasTyC Γ Skip
+
+  | Ty_Assign : ∀ {Γ x a},
+                HasTyA Γ a (Γ x) ->
+                HasTyC Γ (x <~ a)
+
+  | Ty_Seq    : ∀ {Γ c1 c2},
+                HasTyC  Γ c1 -> HasTyC Γ c2 ->
+                HasTyC Γ (c1 ;; c2)
+
+  | Ty_If     : ∀ {Γ b c1 c2},
+                HasTyB Γ b -> HasTyC Γ c1 -> HasTyC Γ c2 ->
+                HasTyC Γ (IF b THEN c1 ELSE c2)
+
+  | Ty_While  : ∀ {Γ b c},
+                HasTyB Γ b -> HasTyC Γ c  ->
+                HasTyC Γ (WHILE b DO c END)
+
+notation:10 Γ " ⊢ " c  => HasTyC Γ c
+
+-- Yay for syntax directed!
+example : Γᵢ ⊢ "x" <~ Ic 3 ;; "y" <~ (V "x") + (Ic 4) := by
+  repeat constructor
+
+/- @@@
+
+## Type Soundness
+
+Ok great, so we made up a system of "type checking" rules.
+
+But how do we know the rules are *sensible* or *meaningful* ?
+
+How do we know the rules actually tell us something about the programs *execution*?
+
+That is, right now we have defined *two* semantics for FIMP:
+
+- **Dynamic Semantics** i.e. how the programs **run** via the `SmallStep` operational semantics; and
+
+- **Static Semantics** i.e. how the programs **type-check** via the `HasTy` rules.
+
+How can we *relate* or *connect* these two descriptions of program behavior?
+
+
+@@@ -/
+
+
+@[simp] def type(v: Val) : Ty := match v with
+  | Iv _ => TInt
+  | Fv _ => TFloat
+
+@[simp] def Wf (Γ: Env) (s: State) : Prop :=
+  ∀ x, Γ x = type (s x)
+
+notation:10 Γ " ⊧ " s  => Wf Γ s
+
+
+theorem arith_preservation : ∀ { Γ a τ s v },
+  (Γ ⊧ s) -> (Γ ⊢ a : τ) -> Taval a s v -> type v = τ
+  := by
+  intros Γ a τ s v G_s G_a_t a_s_v
+  induction G_a_t generalizing v
+  . case Ty_Ic i => cases a_s_v; simp_all
+  . case Ty_Fc f => cases a_s_v; simp_all
+  . case Ty_V x  => cases a_s_v; simp_all
+  . case Ty_AddI a1 a2 _ _ ih1 _ =>
+    cases a_s_v
+    . simp_all
+    . rename_i _ _ av1 _; apply (ih1 av1)
+  . case Ty_AddF a1 a2 _ _ ih1 _ =>
+    cases a_s_v
+    . rename_i _ _ av1 _; apply (ih1 av1)
+    . simp_all
+
+@[simp] def ty_val (t:Ty) (v:Val) : Prop :=
+  match t with
+  | TInt => ∃ n, v = Iv n
+  | TFloat => ∃ n, v = Fv n
+
+theorem arith_preservation_val : ∀ { Γ s a τ v },
+  (Γ ⊧ s) -> (Γ ⊢ a : τ) -> Taval a s v -> ty_val τ v
+  := by
+  intros Γ s a τ v _ _ _
+  have hv : type v = τ := by apply arith_preservation; repeat assumption
+  cases v <;> simp_all [<-hv]
+
+theorem add_step : ∀ {Γ a1 a2 s v1 v2 τ},
+  (Γ ⊧ s) -> (Γ ⊢ a1 : τ) -> (Γ ⊢ a2 : τ) ->
+  (Taval a1 s v1) -> (Taval a2 s v2) ->
+  ∃ v, Taval (a1 + a2) s v
+  := by
+  intros Γ a1 a2 s v1 v2 τ gs gt1 gt2 av1 av2
+  have h1' : ty_val τ v1 := by
+    apply arith_preservation_val
+    assumption; apply gt1; assumption
+  have h2' : ty_val τ v2 := by
+    apply arith_preservation_val
+    assumption; apply gt2; assumption
+  cases τ
+  . case TInt =>
+    cases h1'; cases h2'; simp_all; constructor; apply T_AddI; repeat assumption
+  . case TFloat =>
+    cases h1'; cases h2'; simp_all; constructor; apply T_AddF; repeat assumption
+
+theorem add_progress: ∀ {Γ a1 a2 τ s},
+  (Γ ⊧ s) -> (Γ ⊢ a1 : τ) -> (Γ ⊢ a2 : τ) ->
+  (∃ v1, Taval a1 s v1) -> (∃ v2, Taval a2 s v2) ->
+  ∃ v, Taval (a1 + a2) s v
+  := by
+  intros Γ a1 a2 τ s gs g1 g2 av1 av2
+  cases av1; cases av2; apply add_step; repeat assumption
+
+theorem arith_progress: ∀ { Γ a τ s },
+  (Γ ⊧ s) -> (Γ ⊢ a : τ) ->  ∃ v, Taval a s v  := by
+  intros Γ a τ s G_s G_a_t
+  induction G_a_t
+  . case Ty_Ic i => repeat constructor
+  . case Ty_Fc f => repeat constructor
+  . case Ty_V x  => repeat constructor
+  . case Ty_AddI => apply add_progress; repeat assumption
+  . case Ty_AddF => apply add_progress; repeat assumption
+
+
+-- almost same as `add_step` ...
+
+theorem less_step : ∀ {Γ a1 a2 s v1 v2 τ},
+  (Γ ⊧ s) -> (Γ ⊢ a1 : τ) -> (Γ ⊢ a2 : τ) ->
+  (Taval a1 s v1) -> (Taval a2 s v2) ->
+  ∃ v, Tbval (a1 << a2) s v
+  := by
+  intros Γ a1 a2 s v1 v2 τ gs gt1 gt2 av1 av2
+  have h1' : ty_val τ v1 := by
+    apply arith_preservation_val
+    assumption; apply gt1; assumption
+  have h2' : ty_val τ v2 := by
+    apply arith_preservation_val
+    assumption; apply gt2; assumption
+  cases τ
+  . case TInt =>
+    cases h1'; cases h2'; simp_all; constructor; apply T_LessI; repeat assumption
+  . case TFloat =>
+    cases h1'; cases h2'; simp_all; constructor; apply T_LessF; repeat assumption
+
+theorem bool_progress: ∀ { Γ s } { b : Bexp },
+  (Γ ⊧ s) -> (Γ ⊢ b) -> ∃ v, (Tbval b s v)
+  := by
+  intros Γ s b Gs Gb
+  induction Gb
+  . case Ty_Bc v =>
+    repeat constructor
+  . case Ty_Not b' gb' ih =>
+    cases ih
+    repeat constructor
+    assumption
+  . case Ty_And b1 b2 Gb1 Gb2 ih1 ih2 =>
+    cases ih1; cases ih2
+    repeat constructor
+    repeat assumption
+  . case Ty_Less a1 a2 τ Ga1 Ga2 =>
+    have h1 : ∃ v1, Taval a1 s v1 := by apply arith_progress; repeat assumption
+    have h2 : ∃ v2, Taval a2 s v2 := by apply arith_progress; repeat assumption
+    cases h1; cases h2; apply less_step; repeat assumption
+
+-------------------
+
+theorem update_ty : ∀ { Γ s x v },  (Γ ⊧ s) -> (type v = Γ x) -> (Γ ⊧ s [x := v]) := by
+  intros Γ s x v v_ty_x wf_s y
+  by_cases (y = x) <;> simp_all         --
+
+theorem state_preservation : ∀ { Γ } { c c' : Com } { s s' },
+  (Γ ⊢ c) -> (Γ ⊧ s) -> Step (c, s) (c', s') -> (Γ ⊧ s')
+  := by
+  intros Γ c c' s s' ty_c wf_s step_c_c'
+  induction ty_c generalizing c' s <;> cases step_c_c' <;> repeat trivial
+  . case Ty_Assign.Assign => apply update_ty; trivial; apply arith_preservation; repeat trivial
+  . case Ty_Seq.Seq2      => rename_i ih1 _ _ _; apply ih1; repeat trivial
+
+theorem preservation : ∀ { Γ } { c c' : Com } { s s' : State },
+  (Γ ⊧ s) -> (Γ ⊢ c) -> Step (c, s) (c', s') -> (Γ ⊢ c')
+  := by
+  intros Γ c c' s s' wf_s ty_c step
+  induction ty_c generalizing c' s s' <;> cases step <;> repeat trivial
+  . case Ty_Assign.Assign => constructor
+  . case Ty_Seq.Seq2      => rename_i ih _ _ _; constructor; apply ih; repeat trivial
+  . case Ty_While         => repeat (constructor <;> repeat trivial)
+
+----------------
+
+theorem progress1 : ∀ { Γ s } { c : Com},
+  (Γ ⊧ s) -> (Γ ⊢ c) ->  ¬ (c = Skip) -> ∃ c' s', Step (c, s) (c', s')
+  := by
+  intros Γ s c wf_s ty_c not_skip
+  induction ty_c <;> repeat trivial
+  -- assign
+  . case Ty_Assign x a a_ty =>
+    cases (arith_progress wf_s a_ty)
+    repeat constructor
+    repeat assumption
+  -- seq
+  . case Ty_Seq    =>
+    rename_i c1 c2 c1_ty c2_ty ih1 ih2
+    by_cases (c1 = Skip)
+    . case pos =>
+      apply Exists.intro; apply Exists.intro
+      simp_all
+      apply Step.Seq1
+    . case neg c1_notskip =>
+      cases (ih1 c1_notskip)
+      rename_i c1' step1'
+      cases step1'
+      apply Exists.intro; apply Exists.intro;
+      apply Step.Seq2
+      repeat trivial
+  -- if
+  . case Ty_If     =>
+    rename_i b c1 c2 b_ty _ _ _ _
+    cases (bool_progress wf_s b_ty)
+    rename_i bv hbv
+    cases bv
+    . case intro.false =>
+      apply Exists.intro; apply Exists.intro;
+      apply Step.IfFalse; assumption
+    . case intro.true =>
+      apply Exists.intro; apply Exists.intro;
+      apply Step.IfTrue; assumption
+  -- while
+  . case Ty_While =>
+    apply Exists.intro; apply Exists.intro;
+    apply Step.While
+
+abbrev Steps := star Step
+
+theorem progress : ∀ { Γ } { c c' : Com } { s s' : State},
+  (Γ ⊧ s) -> (Γ ⊢ c) -> Steps (c, s) (c', s') -> ¬ (c' = Skip) ->
+  ∃ c'' s'', Step (c', s') (c'', s'')
+  := by
+  intros Γ c c' s s' wf_s ty_c steps not_skip
+  generalize h : (c, s)   = cs at steps --- this is ANF / Nico's tip
+  generalize h : (c', s') = cs' at steps --- this is ANF / Nico's tip
+  induction steps generalizing Γ c s c' s'
+  . case refl =>
+    rename_i h1
+    cases h1
+    cases h
+    apply (progress1 wf_s ty_c not_skip)
+  . case step =>
+    rename_i cs1 cs2 cs3 step1 step_rest ih hh
+    cases cs2
+    rename_i c2 s2
+    cases h
+    cases hh
+    have ty_c2 : HasTyC Γ c2 := by apply (preservation wf_s ty_c step1)
+    have wf_s2 : Wf Γ s2     := by apply (state_preservation ty_c wf_s step1)
+    apply (ih wf_s2 ty_c2 not_skip)
+    repeat trivial
